

Exercises in Basic Algebra

1) Expand the following expressions:

a) $3x(yz - y^2 + x^2)$

b) $(3c - d)(a + b)$

c) $(c + d)^2$

d) $(c - d)^2$

e) $\left(\frac{1}{a} + a\right)^2$

f) $(c + d + e)^2$

g) $(c + d - e)^2$

2) Simplify the following expressions:

a) $(x + y)^2 - (x - y)^2$

b) $(s - t)(s + t) + \left(t - \frac{s^2}{2t}\right)^2$

c) $\frac{x^2 + 2xy + y^2}{x + y}$

d) $\frac{a^2 - b^2}{a - b}$

e) $\frac{ac^2 - az^2}{c + z}$

3) Simplify the following:

a) $s^2 s^4$

b) $\frac{w^5}{w^3}$

c) $x^{2.5} \sqrt{x}$

d) $(d^5)^8$

e) $\frac{(a^6)^{\frac{1}{3}}}{a}$

f) g^0

g) $z^{-2} \sqrt{z^3}$

h) $\frac{(ab)^3}{a^3}$

i) $(xy)^4 (yz)^{-3} (xz)^2$

4) Write out the following sums without a summation notation (without a Σ):

a) $\sum_{k=1}^3 3k$

b) $\sum_{k=4}^5 3k$

c) $\sum_{j=0}^3 j^2$

d) $\sum_{m=5}^8 (m - 3)$

e) $\sum_{l=-3}^1 (l^2 + 1)$

f) $\sum_{k=2}^4 \frac{k + 2}{k - 1}$

5) Calculate the following arithmetic sums:

a) $\sum_{k=1}^{10} k$

b) $\sum_{k=1}^{10} 2k$

c) $\sum_{k=1}^4 3$

d) $\sum_{k=1}^4 (3 + k)$

6) Calculate the following geometric sums:

a) $\sum_{k=0}^3 2^k$

b) $\sum_{k=-1}^2 3^k$

c) $\sum_{j=0}^4 \left(\frac{1}{3}\right)^j$

d) $\sum_{j=0}^{\infty} \left(\frac{1}{3}\right)^j$

e) $\sum_{k=1}^4 (-2)^k$

f) $\sum_{m=0}^{\infty} (-0.2)^m$

g) $\sum_{k=1}^3 2 \cdot 3^k$

h) $\sum_{j=0}^{\infty} 3 \cdot 0.5^j$

7) Solve the following equations:

a) $x + 3 = 8$

b) $4x - 3 = 2x + 3$

c) $\frac{3+x}{x-1} = 2$

d) $3x = 2x$

e) $x - 2 = \frac{-4+x}{3}$

8) Solve the following equations:

a) $a^2 - 4a + 3 = 0$

b) $x^2 - 2x - 3 = 0$

c) $4x + 6 = 2x^2$

d) $x - 2 = \frac{3}{x-4}$

e) $\frac{y^2}{3} + 2y = -3$

9) Calculate the following:

a) $(3 + 4i) + (1 - 2i)$

b) $(3 + 4i)(1 - 2i)$

c) $(3 + 4i)(3 - 4i)$

Answers

- 1) a) $3xyz - 3xy^2 + 3x^3$ b) $3ac + 3bc - ad - bd$ c) $c^2 + 2cd + d^2$
d) $c^2 - 2cd + d^2$ e) $\frac{1}{a^2} + 2 + a^2$
f) $c^2 + d^2 + e^2 + 2cd + 2ce + 2de$ g) $c^2 + d^2 + e^2 + 2cd - 2ce - 2de$
- 2) a) $4xy$ b) $\frac{s^4}{4t^2}$ c) $x + y$
d) $a + b$ e) $a(c - z)$
- 3) a) s^6 b) w^2 c) x^3
d) d^{40} e) a f) 1
g) $z^{-\frac{1}{2}} = \frac{1}{\sqrt{z}}$ h) b^3 i) $x^6 y z^{-1}$
- 4) a) $3 + 6 + 9$ b) $12 + 15$ c) $0 + 1 + 4 + 9$
d) $2 + 3 + 4 + 5$ e) $10 + 5 + 2 + 1 + 2$ f) $\frac{4}{1} + \frac{5}{2} + \frac{6}{3}$
- 5) a) 55 b) 110 c) 12
d) 22
- 6) a) 15 b) $\frac{40}{3} = 13\frac{1}{3}$ c) $\frac{121}{81} \approx 1.4938$
d) $3/2 = 1.5$ e) 10 f) $\frac{1}{1.2} = \frac{10}{12} = \frac{5}{6}$
g) 78 h) 6
- 7) a) $x = 5$ b) $x = 3$ c) $x = 5$
d) $x = 0$ e) $x = 1$
- 8) a) $a = 2 \pm 1 \Rightarrow a_1 = 1, a_2 = 3$ b) $x_1 = -1, x_2 = 3$ c) $x_1 = -1, x_2 = 3$
d) $x_1 = 1, x_2 = 5$ e) $y = -3$
- 9) a) $4 + 2i$ b) $11 - 2i$ c) 25